@prefix : <example.org/ontologies/games> .
@prefix schema: <https://schema.org/docs/schema.html> .
@prefix rdf: <http://www.w3.org/1999/02/22-rdf-syntax-ns#> .
@prefix rdfs: <http://www.w3.org/2000/01/rdf-schema#> .
@prefix event: <http://motools.sourceforge.net/event/event.html>.
@prefix xsd: <http://www.w3.org/2001/XMLSchema#> .

#TO DO remove?
@prefix owl: <http://www.w3.org/2002/07/owl#> .

#########################
# Classes         
#########################
:GameCompany a rdfs:class;
			rdfs:subClassOf schema:Corporation;
			rdfs:comment "Company that manufactures or provides service related to games."@en;
			rdfs:label "Game company"@en.

:Controller a rdfs:class;
			rdfs:subClassOf schema:Thing;
			rdfs:comment "Tool used to give input from user to game."@en;
			rdfs:label "Game controller"@en.

:Intention a rdfs:class;
			rdfs:subClassOf schema:Thing;
			rdfs:comment "Intention of the game developed."@en;
			rdfs:label "Game intention"@en.

:Game a rdfs:class;
		rdfs:subClassOf schema:VideoGame;
		rdfs:comment "An electronic game."@en;
		rdfs:label "Electronic Game"@en.

:Media a rdfs:class;
		rdfs:subClassOf schema:MediaObject;
		rdfs:comment "Media format to distribute games."@en;
		rdfs:label "Game Media"@en.

:Platform a rdfs:class;
		rdfs:subClassOf schema:Thing;
		rdfs:comment "Platform on which the game is displayed or ran on."@en;
		rdfs:label "Game Platform"@en.

:Console a rdfs:class;
		rdfs:subClassOf :Platform;
		rdfs:comment "Tool used to run a game."@en;
		rdfs:label "Game Console"@en.

:Stream a rdfs:class;
		rdfs:subClassOf :Platform;
		rdfs:comment "Service provider to watch gaming content."@en;
		rdfs:label "Game Streaming"@en.

:Creator a rdfs:class;
		rdfs:subClassOf foaf:Person;
		rdfs:comment "A person who works on the game's developement."@en;
		rdfs:label "Game creator"@en.

:User a rdfs:class;
		rdfs:subClassOf foaf:Person;
		rdfs:comment "A person who plays the game."@en;
		rdfs:label "Gamer"@en.

:Conference a rdfs:class;
			rdfs:subClassOf event:Event;
			rdfs:comment "Event dedicated for the gaming industry."@en;
			rdfs:label "Game conference"@en.

:GamePlayerMode a rdfs:class;
			rdfs:subClassOf schema:Thing;
			rdfs:comment "Number of player in the game."@en;
			rdfs:label "Game player mode"@en.

:GameViewMode a rdfs:class;
			rdfs:subClassOf schema:Thing;
			rdfs:comment "The way how a player will see the game."@en;
			rdfs:label "Game view mode"@en.

:GameGenre a rdfs:class;
		rdfs:subClassOf schema:Thing;
		rdfs:comment "The game genre."@en.
		rdfs:label "Game genre"@en.

#########################
# Data Properties         
#########################

# Game company
:website a rdf:Property;
		rdfs:label "Website"@en;
		rdfs:comment "Company's website"@en;
		rdfs:domain :GameCompany;
		rdfs:range xsd:string.

:country a rdf:Property;
	rdfs:label "country"@en;
	rdfs:comment "Origin country of game"@en;
	rdfs:domain :GameCompany;
	rdfs:range xsd:string.

# User
:username a rdf:Property;
	rdfs:label "Name"@en;
	rdfs:comment "Gamer's username"@en;
	rdfs:domain :User;
	rdfs:range xsd:string.

# Stream
:duration a rdf:Property;
	rdfs:label "Duration"@en;
	rdfs:comment "Streaming duration"@en;
	rdfs:domain :Stream;
	rdfs:range xsd:duration.

# Media
:size a rdf:Property;
	rdfs:label "Size"@en;
	rdfs:comment "Media size"@en;
	rdfs:domain :Media;
	rdfs:range xsd:nonNegativeInteger.

# Game
:releaseDate a rdf:Property;
	rdfs:label "release date"@en;
	rdfs:comment "release date of a game"@en;
	rdfs:domain :Game;
	rdfs:range xsd:dateTime.

:price a rdf:Property;
	rdfs:label "price"@en;
	rdfs:comment "game price"@en;
	rdfs:domain :Game;
	rdfs:range xsd:nonNegativeInteger.

#########################
# Object Properties         
#########################

# Game
:GOwnedBy a rdf:Property;
		rdfs:label "owned by"@en;
		rdfs:comment "Owned by a company"@en;
		rdfs:domain :Game;
		rdfs:range :GameCompany.

:hasPlayerMode a rdf:Property;
				rdfs:label "has player mode"@en;
				rdfs:comment "has player mode"@en;
				rdfs:domain :Game;
				rdfs:range :GamePlayerMode.

:hasViewMode a rdf:Property;
			rdfs:label "has view mode"@en;
			rdfs:comment "has view mode"@en;
			rdfs:domain :Game;
			rdfs:range :GameViewMode.	

:hasGenre a rdf:Property;
			rdfs:label "has genre"@en;
			rdfs:comment "has genre"@en;
			rdfs:domain :Game;
			rdfs:range :GameGenre.

:hasIntent a rdf:Property;
			rdfs:label "has intent"@en;
			rdfs:comment "has intent"@en;
			rdfs:domain :Game;
			rdfs:range :Intention.

:publishedBy a rdf:Property;
			rdfs:label "published by"@en;
			rdfs:comment "game is published by a company"@en;
			rdfs:domain :Game;
			rdfs:range :GameCompany.

:playOn a rdf:Property;	
		rdfs:label "play on"@en;
		rdfs:comment "game can be played on"@en;
		rdfs:domain :Game;
		rdfs:range :Console.

:streamOn a rdf:Property;
		rdfs:label "stream on"@en;
		rdfs:comment "game can be streamed on"@en;
		rdfs:domain :Game;
		rdfs:range :Stream.

:playedWith a rdf:Property;
			rdfs:label "played with"@en;
			rdfs:comment "game can be played with"@en;
			rdfs:domain :Game;
			rdfs:range :Controller.

:format a rdf:Property;
		rdfs:label "format"@en;
		rdfs:comment "format of game"@en;
		rdfs:domain :Game;
		rdfs:range :Media.

# Platform
:POwnedBy a rdf:Property;
		rdfs:label "owned by"@en;
		rdfs:comment "Owned by a company"@en;
		rdfs:domain :Platform;
		rdfs:range :GameCompany.

# Console
:usesController a rdf:Property;
				rdfs:label "uses controller"@en;
				rdfs:comment "console uses specific controller"@en;
				rdfs:domain :Console;
				rdfs:range :Controller.

# User
:usesService a rdf:Property;
			rdfs:label "uses service"@en;
			rdfs:comment "User uses specific service"@en;
			rdfs:domain :User;
			rdfs:range :Platform.

# Creator
:workOn a rdf:Property;
		rdfs:label "work on"@en;
		rdfs:comment "creator work on a game"@en;
		rdfs:domain :Creator;
		rdfs:range :Game.

# Conference
:hostBy a rdf:Property;
		rdfs:label "host by"@en;
		rdfs:comment "event host by company"@en;
		rdfs:domain :Conference;
		rdfs:range :GameCompany.

# REMOVE EVERYTHING UNDER THIS LINE!!!!


#########################
# Corporations
#########################

# :Tencent_Games a schema:Corporation ;
# 	             rdfs:label "Tencent Games" ;
#                  rdfs:comment "Tencent is a Chinese multinational technology conglomerate holding company";
#                  p:url "https://www.tencent.com/";
# 	             schema:countryOfOrigin db:China .

# :Sony a schema:Corporation ;
# 	    rdfs:label "Sony Interactive Entertainment" ;
#         rdfs:comment "Sony Interactive Entertainment is a multinational video game and digital entertainment company.";
#         p:url "https://www.sie.com/en/index.html";
# 	    schema:countryOfOrigin db:Japan .

# :Apple a schema:Corporation ;
# 	     rdfs:label "Apple" ;
#          rdfs:comment "Apple Inc. is an American multinational technology company headquartered in Cupertino, California, that designs, develops and sells consumer electronics, computer software, and online services.";
#          p:url "https://www.apple.com/";
# 	     schema:countryOfOrigin db:United_States .

# :EA a schema:Corporation ;
# 	     rdfs:label "Electronic Arts" ;
#          rdfs:comment "Electronic Arts Inc. (EA) is an American video game company headquartered in Redwood City, California.";
#          p:url "https://www.ea.com/";
# 	     schema:countryOfOrigin db:United_States .

#########################
# Controllers
#########################

# :gamepads a vg:Controller ;
#             rdfs:label "gamepads";
# 			rdfs:comment "A gamepad, is a type of game controller held in two hands, where the fingers (especially thumbs) are used to provide input" .
# :joysticks a vg:Controller ;
#             rdfs:label "joysticks" ;
# 			rdfs:comment "A joystick is an input device consisting of a stick that pivots on a base and reports its angle or direction to the device it is controlling".
# :touchscreen a vg:Controller ;
#             rdfs:label "touchscreen";
# 			rdfs:comment "A touchscreen is an input and output device and normally layered on the top of an electronic visual display of an information processing system".
# :motion_sensor a vg:Controller ;
#             rdfs:label "motion sensor";
# 			rdfs:comment "A motion detector is an electrical device that utilizes a sensor to detect nearby motion".



#########################
# Game intentions
#########################

# :casual_gaming a vg:Intention;
# 				rdfs:label "casual gaming";
# 				rdfs:comment "Casual games are designed for easy of accessibility, simple to understand gameplay and quick to grasp rule sets, and aimed at mass market audience, as opposed to a hardcore game".
# :educational_gaming a vg:Intention;
# 				rdfs:label "educational gaming";
# 				rdfs:comment "Education software has been used in homes and classrooms to help teach children and students".
# :serious_gaming a vg:Intention 
# 				rdfs:label "serious gaming";
# 				rdfs:comment "Further extending from educational games, serious games are those where the entertainment factor may be augmented, overshadowed, or even eliminated by other purposes for the game".


#########################
# Game media
#########################

# :physical a vg:Game_media ;
# 			rdfs:label "physical";
# 			rdfs:comment "Games that are sold or given in a physical format. eg, CD, flash memory";
# 			p:type  (db:CD db:flash_memory).
# :digital a db:game_media ;
# 			rdfs:label "digital";
# 			rdfs:comment "Games that are sold or given in a digital format. eg, downloadable content";
# 			p:type db:downloadable_content .

#########################
# Games
#########################

# :game1 a vg:Game;
# 		rdfs:label "Halo Wars 2";
# 		event:time "2017"^^xsd:gYear.

# :game2 a vg:Game;
# 		rdfs:label "Gears of War 4";
# 		event:time "2016"^^xsd:gYear.

# :game3 a vg:Game;
# 		rdfs:label "Marvel's Spider-Man: Miles Morales";
# 		event:time "2020"^^xsd:gYear.

# :game4 a vg:Game;
# 		rdfs:label "Demon’s Souls";
# 		event:time "2020"^^xsd:gYear.

# :game5 a vg:Games;
# 		rdfs: label "RuneScape";
# 		event:time "2001"^^xsd:gYear.

# :game6 a vg:Games;
# 		rdfs: label "MapleStory";
# 		event:time "2003"^^xsd:gYear;

# :game7 a vg:Games;
# 		rdfs: label "Animal Crossing: New Horizons";
# 		event:time "2020"^^xsd:gYear.

# :game8 a vg:Games;
# 		rdfs: label "Pokémon Sword and Shield";
# 		event:time "2019"^^xsd:gYear;

# :game9 a vg:Games;
# 		rdfs: label "Candy Crush Saga";
# 		event:time "2012"^^xsd:gYear.

# :game10 a vg:Games;
# 		rdfs: label "Flappy Bird";
# 		event:time "2013"^^xsd:gYear;

#########################
# Game consoles
#########################

# vg:Console rdfs:subClassOf vg:Platform .

# :Xbox_One a vg:Console ;
# 		rdfs:label "xbox one";
# 		rdfs:comment "The Xbox One is a home video game console developed by Microsoft.";
# 		p:hasGame :game1, :game2.

# :Playstation5 a vg:Console ;
# 		rdfs:label "Playsation 5";
# 		rdfs:comment "The PlayStation 5 (PS5) is an upcoming home video game console developed by Sony Interactive Entertainment";
# 		p:hasGame :game3, :game4.

# :PC a vg:Console ;
# 		rdfs:label "Personnal computer";
# 		rdfs:comment "A personal computer (PC) is a multi-purpose computer whose size, capabilities, and price make it feasible for individual use";
# 		p:hasGame :game5, :game6.

# :Switch a vg:Console ;
# 		rdfs:label "Nintendo Switch";
# 		rdfs:comment "The Nintendo Switch is a video game console, developed by Nintendo and released worldwide";
# 		p:hasGame :game7, :game8.

# :Mobile a vg:Console ;
# 		rdfs:label "Mobile device";
# 		rdfs:comment "A mobile device is a computer small enough to hold and operate in the hand.";
# 		p:hasGame :game9, :game10.


#########################
# Game streaming platforms
#########################

# vg:Streaming_platform rdfs:subClassOf vg:Platform .

# :Youtube a vg:Streaming_platform ;
# 		rdfs:label "Youtube";
# 		rdfs:comment "YouTube is an American online video-sharing platform.";
# 		p:url "https://www.youtube.com/" .
# :Twitch a vg:Streaming_platform ;
# 		rdfs:label "Twitch";
# 		rdfs:comment "Twitch is a video live streaming service operated by Twitch Interactive, a subsidiary of Amazon.";
# 		p:url "https://www.twitch.tv/" .
# :Mixer a vg:Streaming_platform ;
# 		rdfs:label "Mixer";
# 		rdfs:comment "Mixer was an American video game live streaming platform.";
# 		p:url "https://www.facebook.com/fbgaminghome/blog/welcome-mixer-facebook-gaming" .

#########################
# People
#########################

# vg:Creator rdfs:subClassOf foaf:Person .
# :Developer a vg:Creator;
# 			rdfs:label "Developer";
# 			rdfs:comment "A video game developer is a software developer specializing in video game development – the process and related disciplines of creating video games".
# :GameDesigner a vg:Creator;
# 			rdfs:label "Game designer";
# 			rdfs:comment "A game designer apply design and aesthetics to create a game for entertainment or for educational." .
# :SoundProducer a vg:Creator;
# 			rdfs:label "Sound producer";
# 			rdfs:comment "A sound producer simply operates the technology employed in a recording." .


# vg:User rdfs:subClassOf foaf:Person .
# :Casual_User a vg:User;
# 			rdfs:label "casual user";
# 			rdfs:comment "Type of gamer who usually plays non-competitive games".
# :Hardcore_User a vg:User;
# 			rdfs:label "hardcore user";
# 			rdfs:comment "Type of gamer who usually plays competitive games".
# :Professional_User a vg:User;
# 			rdfs:label "professional user";
# 			rdfs:comment "Type of gamer whose full time job is playing games and will usually partipate in Esports events.".


#########################
# Conferences
#########################

# :E3 a vg:Conference ;
#     rdfs:label "Electronic Entertainment Expo" ;
#     event:time "2021-06-15"^^xsd:date .
# :Dream_Hack a vg:Conference ;
#     rdfs:label "DreamHack" ;
#     event:time "2020-11-26"^^xsd:date .
# :GDC a vg:Conference .
#     rdfs:label "Game Developers Conference" ;
#     event:time "2021-06-19"^^xsd:date .

#########################
# Player Modes
#########################

# :Multiplayer a vg:Player_Mode .
# :SingplePlayer a vg:Player_Mode .
# :Coop a vg:Player_Mode .


#########################
# View Modes
#########################

# db:Top_Down a vg:View_Mode .
# db:Side_Scroller a vg:View_Mode .
# db:First_Person a vg:View_Mode .
# db:Third_Person a vg:View_Mode .


#########################
# Genres
#########################

# db:Survival a vg:Genre .
# db:Platformer a vg:Genre .
# db:Shooter a vg:Genre .
# db:Metroidvania a vg:Genre .

#########################
# Video game
#########################

# vg:Video_Game p:publishedBy db:Tencent_Games .
# vg:Video_Game p:publishedBy db:Sony .
# vg:Video_Game p:publishedBy db:Apple .

# vg:Video_Game p:developedBy db:Electr .
# vg:Video_Game p:developedBy db:Sony .
# vg:Video_Game p:developedBy db:Apple .

